Further work on caching.

examples/CacheADT.v
@@ -1,10 +1,6 @@
 Require Import String Omega List FunctionalExtensionality Ensembles
         Computation ADT ADTRefinement ADTNotation BuildADTRefinements.
 
-Open Scope ADT.
-Open Scope ADTSig.
-Open Scope string.
-
 Section CacheADT.
 
   Variable Key : Type.
@@ -21,8 +17,9 @@ Section CacheADT.
   Definition EnsembleInsert  {A} (a : A) (ens : Ensemble A) (a' : A)
     : Prop := a' = a \/ ens a'.
 
-  Definition SubEnsembleInsert {A} (a : A) (ens ens' : Ensemble A) (a' : A)
-  : Prop := ens' a' -> EnsembleInsert a ens a'.
+  Definition SubEnsembleInsert {A} (a : A) (ens ens' : Ensemble A)
+  : Prop :=
+    forall (a' : A), ens' a' -> EnsembleInsert a ens a'.
 
   Definition EnsembleRemove
              (k : Key)
@@ -54,7 +51,7 @@ Section CacheADT.
           ret (fun _ => False),
         meth "AddKey" (r : rep, kv : Key * Value) : bool :=
             { r' | (usedKey r (fst kv) -> snd r' = false) /\
-                   (~ usedKey r (fst kv) -> (SubEnsembleInsert kv r (fst r') kv)
+                   (~ usedKey r (fst kv) -> (SubEnsembleInsert kv r (fst r'))
                                             /\ snd r' = true)},
         meth "UpdateKey" (r : rep, kv : Key * Value) : bool :=
               { r' | (usedKey r (fst kv) -> r' = (EnsembleReplace kv r, true)) /\
@@ -71,6 +68,420 @@ Require Import FMapAVL.
 
 Module StringIndexedMap := FMapAVL.Make String_as_OT.
 Definition MapStringNat := StringIndexedMap.t nat.
+
+Section AddDuplicateKeyStrategies.
+
+  Variable Key : Type.
+  Variable Value : Type.
+
+  (* Two strategies : replace the key*)
+
+  Lemma refine_ReplaceUsedKey
+  : forall (kv : Key * Value)
+           (r : Ensemble (Key * Value)),
+      refine { r' | (usedKey r (fst kv) -> snd r' = false) /\
+                    (~ usedKey r (fst kv) -> (SubEnsembleInsert kv r (fst r'))
+                                             /\ snd r' = true)}
+             (b <- {b | decides b (usedKey r (fst kv))};
+              r' <- { r' | if b then r' = EnsembleReplace kv r
+                                else SubEnsembleInsert kv r r' };
+              ret (r', negb b)).
+  Proof.
+    intros; rewrite refine_pick_decides.
+    f_equiv; unfold pointwise_relation; intros.
+    destruct a.
+    - refine pick eq; rewrite refineEquiv_bind_unit;
+      apply refine_pick_val; reflexivity.
+    - refine pick pair.
+      refine pick eq.
+      simplify with monad laws.
+      f_equiv.
+  Qed.
+
+  Lemma refine_IgnoreUsedKeyInsert
+  : forall (kv : Key * Value)
+           (r : Ensemble (Key * Value)),
+      refine { r' | (usedKey r (fst kv) -> snd r' = false) /\
+                    (~ usedKey r (fst kv) -> (SubEnsembleInsert kv r (fst r'))
+                                             /\ snd r' = true)}
+             (b <- {b | decides b (usedKey r (fst kv))};
+              r' <- { r' | if b then r' = r
+                                else SubEnsembleInsert kv r r' };
+              ret (r', negb b)).
+  Proof.
+    intros; rewrite refine_pick_decides.
+    f_equiv; unfold pointwise_relation; intros.
+    destruct a.
+    - refine pick eq; rewrite refineEquiv_bind_unit;
+      apply refine_pick_val; reflexivity.
+    - refine pick pair.
+      refine pick eq.
+      simplify with monad laws.
+      f_equiv.
+  Qed.
+
+End AddDuplicateKeyStrategies.
+
+Section CacheEvictionStrategies.
+
+  Variable Key : Type.
+  Variable Value : Type.
+
+  Definition CacheADTwMetric_AbsR
+             (or : Ensemble (Key * Value))
+             (nr : Ensemble (Key * (Value * nat)))
+    := forall kv, or (fst kv, fst (snd kv)) <-> nr kv.
+
+  (* First refinement- determine if there is a key to be replaced. *)
+
+  Lemma refine_SubEnsembleInsert
+  : forall (k : Key)
+           (v : Value)
+           (idx : nat)
+           (r : Ensemble (Key * (Value * nat))),
+      refine { r' | (SubEnsembleInsert (k, (v, idx)) r r')}
+             (kv_opt <- {kv_opt | forall kv',
+                                    kv_opt = Some kv' -> r kv'};
+              {r' | r' = match kv_opt with
+                           | Some (kv', _) =>
+                             EnsembleInsert (k, (v, idx))
+                                            (EnsembleRemove kv' r)
+                           | None => EnsembleInsert (k, (v, idx)) r
+                         end} ).
+  Proof.
+    intros; rewrite refine_Pick_Some with
+            (P := r).
+    f_equiv; unfold pointwise_relation; intros.
+    destruct a;
+      [ higher_order_1_reflexivity 
+      | reflexivity ].
+    simpl; intros; refine pick eq;  apply refine_pick_val;
+    destruct b; unfold SubEnsembleInsert, EnsembleInsert,
+                EnsembleRemove; simpl; intros; intuition.
+    simpl; intros; refine pick eq;  apply refine_pick_val;
+    unfold SubEnsembleInsert, EnsembleInsert,
+    EnsembleRemove; simpl; intros; intuition.
+  Qed.
+
+  Lemma refine_pick_KeyToBeReplaced_min
+  : forall (r : Ensemble (Key * (Value * nat))),
+      refine {kv_opt | forall kv',
+                         kv_opt = Some kv' -> r kv'}
+             {kv_opt | forall kv',
+                         kv_opt = Some kv' -> 
+                         (r kv' 
+                          /\ (forall kv'', 
+                                r kv'' -> (snd (snd kv')) <= snd (snd kv'')))
+                             }.
+  Proof.
+    intros; apply refine_pick_pick; intros.
+    eapply H; eauto.
+  Qed.
+
+  Lemma refine_pick_KeyToBeReplaced_max
+  : forall (r : Ensemble (Key * (Value * nat))),
+      refine {kv_opt | forall kv',
+                         kv_opt = Some kv' -> r kv'}
+             {kv_opt | forall kv',
+                         kv_opt = Some kv' -> 
+                         (r kv' 
+                          /\ (forall kv'', 
+                                r kv'' -> (snd (snd kv'')) <= snd (snd kv')))
+                             }.
+  Proof.
+    intros; apply refine_pick_pick; intros.
+    eapply H; eauto.
+  Qed.
+
+
+  Lemma refine_ReplaceUsedKey
+  : forall (kv : Key * Value)
+           (r : Ensemble (Key * Value)),
+      refine { r' | (usedKey r (fst kv) -> snd r' = false) /\
+                    (~ usedKey r (fst kv) -> (SubEnsembleInsert kv r (fst r'))
+                                             /\ snd r' = true)}
+             (b <- {b | decides b (usedKey r (fst kv))};
+              r' <- { r' | if b then r' = EnsembleReplace kv r
+                                else SubEnsembleInsert kv r r' };
+              ret (r', negb b)).
+  Proof.
+    intros; rewrite refine_pick_decides.
+    f_equiv; unfold pointwise_relation; intros.
+    destruct a.
+    - refine pick eq; rewrite refineEquiv_bind_unit;
+      apply refine_pick_val; reflexivity.
+    - refine pick pair.
+      refine pick eq.
+      simplify with monad laws.
+      f_equiv.
+  Qed.
+
+  Lemma refine_IgnoreUsedKeyInsert
+  : forall (kv : Key * Value)
+           (r : Ensemble (Key * Value)),
+      refine { r' | (usedKey r (fst kv) -> snd r' = false) /\
+                    (~ usedKey r (fst kv) -> (SubEnsembleInsert kv r (fst r'))
+                                             /\ snd r' = true)}
+             (b <- {b | decides b (usedKey r (fst kv))};
+              r' <- { r' | if b then r' = r
+                                else SubEnsembleInsert kv r r' };
+              ret (r', negb b)).
+  Proof.
+    intros; rewrite refine_pick_decides.
+    f_equiv; unfold pointwise_relation; intros.
+    destruct a.
+    - refine pick eq; rewrite refineEquiv_bind_unit;
+      apply refine_pick_val; reflexivity.
+    - refine pick pair.
+      refine pick eq.
+      simplify with monad laws.
+      f_equiv.
+  Qed.
+
+
+  Definition BoundedStringCacheADT_AbsR
+             (or nr : Ensemble (Key * Value))
+    := forall kv, (or kv <-> nr kv) /\
+                  (forall kv', nr kv' -> fst kv' = fst kv).
+
+
+
+  Lemma decides_usedKey
+  : forall (or : Ensemble (string * Value))
+           (nr : StringIndexedMap.t Value)
+           (k : string),
+      BoundedStringCacheADT_AbsR or nr ->
+      decides (if StringIndexedMap.find k nr then
+                 true else
+                 false)
+              (usedKey or k).
+  Proof.
+    unfold BoundedStringCacheADT_AbsR, usedKey; intros;
+    pose proof (H k); intuition.
+    find_if_inside; simpl; eauto.
+    intuition; destruct_ex.
+    destruct (H2 _ H0); discriminate.
+  Qed.
+
+  Lemma AbsR_add_EnsembleReplace
+  : forall nr kv or v,
+      BoundedStringCacheADT_AbsR or nr
+      -> StringIndexedMap.find (elt:=Value) (fst kv) nr = Some v
+      -> BoundedStringCacheADT_AbsR
+           (EnsembleReplace kv or)
+           (StringIndexedMap.add (fst kv) (snd kv) nr).
+  Proof.
+    unfold EnsembleReplace, EnsembleRemove,
+    BoundedStringCacheADT_AbsR;
+    intros; intuition.
+    destruct (string_dec k (fst kv)); subst.
+    left.
+    rewrite (StringIndexedMap.find_1 (StringIndexedMap.add_1 nr (snd kv) (refl_equal (fst kv))))
+      in *; destruct kv; simpl in *; f_equal; congruence.
+    right; split; eauto.
+    eapply H.
+    eauto using StringIndexedMap.find_1, StringIndexedMap.add_3,
+    StringIndexedMap.find_2.
+    subst; simpl in *.
+    eexists; eauto using StringIndexedMap.find_1, StringIndexedMap.add_1.
+    destruct (string_dec k (fst kv)); subst.
+    eexists; eauto using StringIndexedMap.find_1, StringIndexedMap.add_1.
+    destruct (H k).
+    destruct (H4 _ H3).
+    eauto using StringIndexedMap.find_1, StringIndexedMap.add_2,
+    StringIndexedMap.find_2.
+  Qed.
+
+  Lemma AbsR_add_EnsembleInsert
+  : forall nr kv or,
+      BoundedStringCacheADT_AbsR or nr
+      -> StringIndexedMap.find (elt:=Value) (fst kv) nr = None
+      -> BoundedStringCacheADT_AbsR
+           (fun kv' => kv' = kv \/ or kv')
+           (StringIndexedMap.add (fst kv) (snd kv) nr).
+  Proof.
+    unfold SubEnsembleInsert, BoundedStringCacheADT_AbsR;
+    intros; intuition.
+    destruct (string_dec k (fst kv)); subst.
+    left.
+    rewrite (StringIndexedMap.find_1 (StringIndexedMap.add_1 nr (snd kv) (refl_equal (fst kv))))
+      in *; destruct kv; simpl in *; f_equal; congruence.
+    right.
+    pose proof (H k); intuition.
+    eauto using StringIndexedMap.find_1, StringIndexedMap.add_3,
+    StringIndexedMap.find_2.
+    subst; simpl in *.
+    eexists; eauto using StringIndexedMap.find_1, StringIndexedMap.add_1.
+    destruct (string_dec k (fst kv)); subst.
+    eexists; eauto using StringIndexedMap.find_1, StringIndexedMap.add_1.
+    destruct (H k).
+    destruct (H3 _ H2).
+    eauto using StringIndexedMap.find_1, StringIndexedMap.add_2,
+    StringIndexedMap.find_2.
+  Qed.
+
+  Lemma AbsR_add_EnsembleInsertRemove
+  : forall nr or k kv,
+      BoundedStringCacheADT_AbsR or nr
+      -> StringIndexedMap.find (elt:=Value) (fst kv) nr = None
+      -> BoundedStringCacheADT_AbsR
+           (EnsembleInsert kv (EnsembleRemove k or))
+           (StringIndexedMap.add (fst kv) (snd kv) (StringIndexedMap.remove k nr)).
+  Proof.
+    unfold SubEnsembleInsert, EnsembleRemove,
+    EnsembleInsert, BoundedStringCacheADT_AbsR;
+    intros; intuition.
+    destruct (string_dec k0 (fst kv)); subst.
+    left;
+    rewrite (StringIndexedMap.find_1 (StringIndexedMap.add_1 _ (snd kv) (refl_equal (fst kv))))
+      in H1; destruct kv; simpl in *; f_equal; congruence.
+    right; destruct (string_dec k0 k); subst.
+    elimtype False; eapply StringIndexedMap.remove_1 with (x := k); eauto.
+    eapply StringIndexedMap.find_2 in H1.
+    eapply StringIndexedMap.add_3 in H1; eauto.
+    unfold StringIndexedMap.In, StringIndexedMap.Raw.In0; eauto.
+    intuition.
+    eapply H.
+    eapply StringIndexedMap.find_1.
+    eapply StringIndexedMap.remove_3; eauto.
+    eapply StringIndexedMap.add_3; clear n0; eauto.
+    eapply StringIndexedMap.find_2; eauto.
+    subst; simpl.
+    eauto using StringIndexedMap.find_1, StringIndexedMap.add_1.
+    destruct (string_dec k0 (fst kv)); subst.
+    eauto using StringIndexedMap.find_1, StringIndexedMap.add_1.
+    destruct (H k0).
+    destruct (H4 _ H3).
+    eexists.
+    eapply StringIndexedMap.find_2 in H5.
+    eapply StringIndexedMap.remove_2 in H5.
+    eapply StringIndexedMap.add_2 in H5; eauto.
+    eapply StringIndexedMap.find_1; eauto.
+    simpl in *; congruence.
+  Qed.
+
+  Definition BoundedStringCacheADT' :
+    Sharpened (@CacheSpec string Value).
+  Proof.
+    unfold CacheSpec; simpl.
+    hone representation using BoundedStringCacheADT_AbsR.
+
+    hone constructor "EmptyCache".
+    {
+      simplify with monad laws.
+      rewrite refine_pick_val with
+      (A := StringIndexedMap.t Value)
+      (a := StringIndexedMap.empty Value).
+      finish honing.
+      unfold BoundedStringCacheADT_AbsR; intros; intuition.
+      eapply (StringIndexedMap.empty_1); eauto.
+      eapply (StringIndexedMap.find_2); eauto.
+    }
+
+    hone method "LookupKey".
+    {
+      simplify with monad laws.
+      refine pick val (StringIndexedMap.find n r_n).
+      simplify with monad laws; simpl.
+      rewrite refine_pick_val by eauto.
+      simplify with monad laws.
+      finish honing.
+      unfold BoundedStringCacheADT_AbsR, ValidLookup in *;
+        intros; pose proof (H0 n); intuition.
+    }
+
+    hone method "UpdateKey".
+    {
+      rewrite refine_pick_decides;
+        simplify with monad laws.
+      rewrite refine_pick_val by eauto using decides_usedKey.
+      simplify with monad laws.
+      eapply refine_if with
+      (b := if StringIndexedMap.find (elt:=Value) (fst n) r_n then true else false).
+      {
+        (* If the Key is used, do this. *)
+        caseEq (StringIndexedMap.find (elt:=Value) (fst n) r_n);
+        try discriminate; simpl.
+        rewrite refineEquiv_pick_eq; simplify with monad laws; simpl.
+        rewrite refine_pick_val by
+          eauto using AbsR_add_EnsembleReplace.
+        simplify with monad laws.
+        reflexivity.
+      }
+      {
+        (* If the Key isn't in the cache, do this. *)
+        caseEq (StringIndexedMap.find (elt:=Value) (fst n) r_n);
+        try discriminate; simpl.
+        erefine pick val (_, _).
+        simplify with monad laws.
+        rewrite refine_pick_val by eauto.
+        simplify with monad laws; simpl; reflexivity.
+      }
+    }
+
+    hone method "AddKey".
+    {
+      rewrite refine_pick_decides;
+      simplify with monad laws.
+      rewrite refine_pick_val by eauto using decides_usedKey.
+      simplify with monad laws.
+      eapply refine_if with
+      (b := if StringIndexedMap.find (elt:=Value) (fst n) r_n then true else false).
+      {
+        (* If the Key is used, do nothing. *)
+        caseEq (StringIndexedMap.find (elt:=Value) (fst n) r_n);
+        try discriminate; simpl.
+        erefine pick val (_, _).
+        simplify with monad laws.
+        rewrite refine_pick_val by eauto.
+        simplify with monad laws; simpl; reflexivity.
+      }
+      {
+        (* If the Key is not used, do this. *)
+        caseEq (StringIndexedMap.find (elt:=Value) (fst n) r_n);
+        try discriminate; simpl.
+        refine pick_pair.
+        setoid_rewrite refineEquiv_pick_eq; simplify with monad laws.
+        (* Check if there is a key worth removing *)
+        etransitivity;
+          [ eapply (refine_Pick_Some (A := StringIndexedMap.t Value * bool)
+                                     (fun kv => StringIndexedMap.find (fst kv) r_n = Some (snd kv)))
+          | ].
+        { (* If so, replace it. *)
+          intros.
+          refine pick val (EnsembleInsert n (EnsembleRemove (fst b) or)).
+          simplify with monad laws; simpl.
+          rewrite refine_pick_val
+            by eauto using AbsR_add_EnsembleInsertRemove.
+          simplify with monad laws.
+          higher_order_1_reflexivity.
+          unfold SubEnsembleInsert, EnsembleInsert, EnsembleRemove; eauto.
+        }
+        {
+          (* If not, do a standard insert. *)
+          refine pick val (EnsembleInsert n or).
+          simplify with monad laws; simpl.
+          rewrite refine_pick_val
+            by eauto using AbsR_add_EnsembleInsert.
+          simplify with monad laws.
+          reflexivity.
+          unfold SubEnsembleInsert, EnsembleInsert, EnsembleRemove; eauto.
+        }
+        (* Here's where we can decide how to pick the element to
+         replace. Picking None lets the cache grow unboundedly. *)
+        refine pick val (@None (StringIndexedMap.key * Value) ).
+        try simplify with monad laws.
+        reflexivity.
+        intuition; try discriminate.
+      }
+
+    }
+
+    finish sharpening.
+
+  Defined.
+
+End BoundedStringCacheADT.
 
 Section BoundedStringCacheADT.
 
@@ -319,7 +730,7 @@ Section BoundedStringCacheADT.
           reflexivity.
           unfold SubEnsembleInsert, EnsembleInsert, EnsembleRemove; eauto.
         }
-        (* Here's where we can decide how to pick the element to 
+        (* Here's where we can decide how to pick the element to
          replace. Picking None lets the cache grow unboundedly. *)
         refine pick val (@None (StringIndexedMap.key * Value) ).
         try simplify with monad laws.
@@ -334,4 +745,3 @@ Section BoundedStringCacheADT.
   Defined.
 
 End BoundedStringCacheADT.
-
