src/Computation.v
@@ -4,3 +4,5 @@ Require Export Computation.SetoidMorphisms.
 Require Export Computation.ReflectiveMonad.
 Require Export Computation.ApplyMonad.
 Require Export Computation.Refinements.General.
+
+Open Scope comp.
